@prefix sh:   <http://www.w3.org/ns/shacl#> .
@prefix skos: <http://www.w3.org/2004/02/skos/core#>.
@prefix dct:  <http://purl.org/dc/terms/>.
@prefix dc:   <http://purl.org/dc/elements/1.1/>.
@prefix rdfs: <http://www.w3.org/2000/01/rdf-schema#>.
@prefix foaf: <http://xmlns.com/foaf/0.1/>.
@prefix dcat: <http://www.w3.org/ns/dcat#> .
@prefix xsd:  <http://www.w3.org/2001/XMLSchema#> .
@prefix :     <http://shacl-play.sparna.fr/shapes-catalog#> .

:shsh a dcat:Dataset ;
  dct:title "SHACL for SHACL" ;
  dct:description "A SHACL shapes graph to validate SHACL shapes graphs." ;
  foaf:isPrimaryTopicOf [
    dct:issued "2020-02-21"^^xsd:date ;
    dct:creator "Thomas Francart" ;
  ] ;
  dcat:distribution [
    dcat:downloadURL <https://www.w3.org/ns/shacl-shacl> ;
    dcat:mediaType <https://www.iana.org/assignments/media-types/text/turtle> ;
  ] ;
  dct:publisher "W3C" ;  
  dcat:keyword "SHACL" ;
  dct:issued "2017-04-04"^^xsd:date ;
  dct:creator "W3C Data Shapes Working Group" ;
  dct:language "en" ;
  dcat:landingPage <https://www.w3.org/TR/shacl/> ;
  dct:isRequiredBy <https://www.w3.org/TR/shacl/> ;
  dct:references <http://www.w3.org/ns/shacl#> ;
.

:shaclplay-catalog a dcat:Dataset ;
  dct:title "SHACL Play! Catalog shapes" ;
  dct:description "The expected structure of the SHACL Play! <a href=\"https://shacl-play.sparna.fr/play/catalog\">Shapes Catalog</a>.";
  foaf:isPrimaryTopicOf [
    dct:issued "2020-01-13"^^xsd:date ;
    dct:creator "Thomas Francart" ;
  ] ;
  dcat:distribution [
    dcat:downloadURL <https://shacl-play.sparna.fr/play/resources/shapes/shacl-play-shapes-catalog.ttl> ;
    dcat:mediaType <https://www.iana.org/assignments/media-types/text/turtle> ;
  ] ;
  dcat:contactPoint <mailto:thomas.francart@sparna.fr> ;
  dct:publisher "Sparna" ;  
  dcat:keyword "SHACL", "SHACL Play!" ;
  dct:issued "2020-01-13"^^xsd:date ;
  dct:creator "Thomas Francart" ;
  dct:language "en" ;
  dcat:landingPage <https://shacl-play.sparna.fr/play/catalog> ;
  dct:isRequiredBy <https://shacl-play.sparna.fr> ;
  dct:references <http://www.w3.org/ns/dcat#>, <http://purl.org/dc/terms/>, <http://xmlns.com/foaf/0.1/> ;
.


:eli a dcat:Dataset ;
  dct:title "ELI Shapes" ;
  dct:description "The <a href=\"https://op.europa.eu/en/web/eu-vocabularies/eli\">European Legislation Idenfitier ontology</a> defines a common data model for exchanging legislation metadata on the web; the primary users of the ELI model are the official legal publishers of EU Member States, and the model can also be used by other organisations. The description of legislation in ELI follows the principles of FRBR.";
  foaf:isPrimaryTopicOf [
    dct:issued "2019-12-01"^^xsd:date ;
    dct:creator "Thomas Francart" ;
  ] ;
  dcat:distribution [
    dcat:downloadURL <https://webgate.ec.europa.eu/eli-validator/shapes/eli-1.2-shapes.ttl> ;
    dcat:mediaType <https://www.iana.org/assignments/media-types/text/turtle> ;
  ] ;
  dcat:distribution [
    dcat:downloadURL <https://webgate.ec.europa.eu/eli-validator/shapes/eli-1.2-shapes.xlsx> ;
    dcat:mediaType <https://www.iana.org/assignments/media-types/application/vnd.ms-excel> ;
  ] ;
  dcat:contactPoint <mailto:thomas.francart@sparna.fr> ;
  dct:publisher "ELI Taskforce" ;  
  dcat:keyword "ELI", "Legislation" ;
  dct:issued "2017-02-01"^^xsd:date ;
  dct:creator "Thomas Francart" ;
  dct:language "en" ;
  dcat:landingPage <https://op.europa.eu/en/web/eu-vocabularies/eli> ;
  dct:isRequiredBy <https://webgate.ec.europa.eu/eli-validator/>, <https://eur-lex.europa.eu/eli-register/about.html> ;
  dct:references <http://data.europa.eu/eli/ontology#> ;
.


:openarchaeo a dcat:Dataset ;
  dct:title "OpenArchaeo Shapes" ;
  dct:description "Model of the <a href=\"http://openarchaeo.huma-num.fr/explorateur/\">OpenArchaeo platform</a>, a subset of the CIDOC-CRM + CRMarchaeo to describe archaelogical sites discoveries, walls, burials, furnitures, stratigraphic units.";
  foaf:isPrimaryTopicOf [
    dct:issued "2019-12-01"^^xsd:date ;
    dct:creator "Thomas Francart" ;
  ] ;
  dcat:distribution [
    dcat:downloadURL <http://openarchaeo.huma-num.fr/federation/resources/shapes/OpenArchaeo-Shapes.ttl> ;
    dcat:mediaType <https://www.iana.org/assignments/media-types/text/turtle> ;
  ] ;
  dcat:distribution [
    dcat:downloadURL <http://openarchaeo.huma-num.fr/federation/resources/shapes/OpenArchaeo-Shapes.xslx> ;
    dcat:mediaType <https://www.iana.org/assignments/media-types/application/vnd.ms-excel> ;
  ] ;
  # dcat:contactPoint <mailto:> ;
  dct:publisher "MASA consortium" ;  
  dcat:keyword "Archaeology", "OpenArchaeo", "CIDOC-CRM" ;
  dct:issued "2019-12-02"^^xsd:date ;
  dct:creator "Thomas Francart" ;
  dct:language "fr" ;
  # dcat:landingPage
  dct:isRequiredBy <http://openarchaeo.huma-num.fr/explorateur/> ;
  dct:references <http://www.cidoc-crm.org/cidoc-crm/>, <http://www.ics.forth.gr/isl/CRMarchaeo/>, <http://www.ics.forth.gr/isl/CRMba/>, <http://www.ics.forth.gr/isl/CRMsci/> ;
.



:scoLOMFR a dcat:Dataset ;
  dct:title "ScoLOMFR Application Profile" ;
  dct:description "Application Profile for the dissemination of the <a href=\"https://www.reseau-canope.fr/scolomfr/accueil.html\">ScoLOMFR</a> in RDF.";
  foaf:isPrimaryTopicOf [
    dct:issued "2020-05-25"^^xsd:date ;
    dct:creator "Thomas Francart" ;
  ] ;
  dcat:distribution [
    dcat:downloadURL <https://gist.githubusercontent.com/tfrancart/cd7af66ba629352f353bec49b76efb98/raw/ScoLOMFR-V6-AP-SHACL.ttl> ;
    dcat:mediaType <https://www.iana.org/assignments/media-types/text/turtle> ;
  ] ;
  #dcat:distribution [
  #  dcat:downloadURL <.xslx> ;
  #  dcat:mediaType <https://www.iana.org/assignments/media-types/application/vnd.ms-excel> ;
  #] ;
  # dcat:contactPoint <mailto:> ;
  dct:publisher "Réseau Canopé" ;  
  dcat:keyword "ScoLOMFR", "LOM", "LOMFR", "Ressources Pédagogiques" ;
  dct:issued "2020-06-30"^^xsd:date ;
  dct:creator "Thomas Francart" ;
  dct:language "fr" ;
  dcat:landingPage <https://www.reseau-canope.fr/scolomfr/accueil.html> ;
  # dct:isRequiredBy <http://openarchaeo.huma-num.fr/explorateur/> ;
  dct:references <http://www.w3.org/2004/02/skos/core#>, <https://www.reseau-canope.fr/scolomfr/ontologie#>, <http://www.w3.org/2008/05/skos-xl#>, <http://www.w3.org/ns/dcat#>, <http://purl.org/dc/terms/>, <http://purl.org/iso25964/skos-thes#>, <http://www.w3.org/ns/prov#> ;
.


:op-skosShapes a dcat:Dataset ;
  dct:title "SKOS Shapes (Office of Publications)" ;
  dct:description """Implements the following SKOS constraint checks: 
- S9	skos:ConceptScheme is disjoint with skos:Concept.  
- S13 : skos:prefLabel, skos:altLabel and skos:hiddenLabel are pairwise disjoint properties. 
- S14	A resource has no more than one value of skos:prefLabel per language tag. 
- S27	skos:related is disjoint with the property skos:broaderTransitive. 
- S37	skos:Collection is disjoint with each of skos:Concept and skos:ConceptScheme.  
- (9.6.4.) SKOS Concepts, Concept Collections and Semantic Relations  
- S46	skos:exactMatch is disjoint with each of the properties skos:broadMatch and skos:relatedMatch. 
- (10.6.2.) Clashes Between Hierarchical (skos:broadMatch skos:narrowMatch) and Associative (skos:relatedMatch, skos:closeMatch, skos:exactMatch) Mappings 
- (B.3.4.2). SKOS+XL Labeling Integrity 
Some warning and few error constraints are also taken from qSKOS validator [https://github.com/cmader/qSKOS/wiki/Quality-Issues#Labeling_and_Documentation_Issues] """ ;
  foaf:isPrimaryTopicOf [
    dct:issued "2020-10-22"^^xsd:date ;
    dct:creator "Thomas Francart" ;
  ] ;
  dcat:distribution [
    dcat:downloadURL <https://op.europa.eu/documents/3938058/5352035/skosShapes.shapes.ttl/6f355b14-6b3e-844a-e05d-1528dd40c4b5?t=1545061378000> ;
    dcat:mediaType <https://www.iana.org/assignments/media-types/text/turtle> ;
  ] ;
  dcat:distribution [
    dcat:downloadURL <https://op.europa.eu/documents/3938058/5352035/swp.html/e3d67af9-640a-ec3b-4b21-7a8ddfbedab9> ;
    dcat:mediaType <https://www.iana.org/assignments/media-types/text/html> ;
  ] ;
  #dcat:distribution [
  #  dcat:downloadURL <.xslx> ;
  #  dcat:mediaType <https://www.iana.org/assignments/media-types/application/vnd.ms-excel> ;
  #] ;
  # dcat:contactPoint <mailto:> ;
  dct:publisher "Office of Publications of the EU" ;  
  dcat:keyword "SKOS", "SKOS-XL" ;
  dct:issued "2020-01-01"^^xsd:date ;
  dct:creator "Office of Publications of the EU" ;
  dct:language "en" ;
  dcat:landingPage <https://op.europa.eu/fr/web/eu-vocabularies/application-profiles> ;
  # dct:isRequiredBy <http://openarchaeo.huma-num.fr/explorateur/> ;
  dct:references <http://www.w3.org/2004/02/skos/core>, <http://www.w3.org/2008/05/skos-xl> ;
.

:lode a dcat:Dataset ;
  dct:title "LODE Shapes from DBPedia Archivo" ;
  dct:description "Set of constraints to validate an ontology so that it can be properly processed by the LODE tool to generate documentation";
  foaf:isPrimaryTopicOf [
    dct:issued "2020-12-07"^^xsd:date ;
    dct:creator "Thomas Francart" ;
  ] ;
  dcat:distribution [
    dcat:downloadURL <https://github.com/dbpedia/archivo/raw/master/shacl-library/LODE.ttl> ;
    dcat:mediaType <https://www.iana.org/assignments/media-types/text/turtle> ;
  ] ;
  #dcat:distribution [
  #  dcat:downloadURL <.xslx> ;
  #  dcat:mediaType <https://www.iana.org/assignments/media-types/application/vnd.ms-excel> ;
  #] ;
  # dcat:contactPoint <mailto:> ;
  dct:publisher "DBPedia Archivo" ;  
  dcat:keyword "OWL", "LODE", "Ontologies" ;
  dct:issued "2020-07-05"^^xsd:date ;
  dct:creator "DBPedia Archivo" ;
  dct:language "en" ;
  dcat:landingPage <https://archivo.dbpedia.org/> ;
  dct:isRequiredBy <https://essepuntato.it/lode/>, <https://github.com/dgarijo/Widoco> ;
  dct:references <http://purl.org/dc/elements/1.1/>, <http://www.w3.org/2002/07/owl#>, <http://www.w3.org/2000/01/rdf-schema#> ;
.

:sparnaturalShaclShapes a dcat:Dataset ;
  dct:title "Sparnatural SHACL configuration profile" ;
  dct:description "Defines the subset of SHACL used to configure <a href=\"https://sparnatural.eu\">Sparnatural</a>. See more details in the <a href=\"http://docs.sparnatural.eu/SHACL-based-configuration\">configuration documentation</a>";
  foaf:isPrimaryTopicOf [
    dct:issued "2023-07-11"^^xsd:date ;
    dct:creator "Thomas Francart" ;
  ] ;
  dcat:distribution [
    dcat:downloadURL <https://xls2rdf.sparna.fr/rest/convert?noPostProcessings=true&url=https%3A%2F%2Fdocs.google.com%2Fspreadsheets%2Fd%2F195NKb43Ck1yPGrIK4H8_HYGw9GTPnbtY%2Fexport%3Fformat%3Dxlsx> ;
    dcat:mediaType <https://www.iana.org/assignments/media-types/text/turtle> ;
  ] ;
  dcat:distribution [
    dcat:downloadURL <https://docs.google.com/spreadsheets/d/195NKb43Ck1yPGrIK4H8_HYGw9GTPnbtY/export?format=xlsx> ;
    dcat:mediaType <https://www.iana.org/assignments/media-types/application/vnd.ms-excel> ;
  ] ;
  dcat:contactPoint <mailto:thomas.francart@sparna.fr> ;
  dct:publisher "Sparna" ;  
  dcat:keyword "Sparnatural", "SHACL", "SPARQL" ;
  dct:issued "2023-07-11"^^xsd:date ;
  dct:creator "Thomas Francart" ;
  dct:language "en" ;
  dcat:landingPage <http://docs.sparnatural.eu/SHACL-based-configuration> ;
  dct:isRequiredBy <https://sparnatural.eu> ;
  dct:references <http://www.w3.org/ns/shacl#>, <http://data.sparna.fr/ontologies/volipi>, <http://datashapes.org/dash#>, <http://www.w3.org/2000/01/rdf-schema#> ;
.

:xkosBpShapesConformance a dcat:Dataset ;
  dct:title "XKOS best practices conformance shapes" ;
  dct:description "Specifies the conformance shapes defined in the <a href=\"http://linked-statistics.github.io/xkos/xkos-best-practices.html\">XKOS Best Practices guide</a>. ";
  foaf:isPrimaryTopicOf [
    dct:issued "2023-07-11"^^xsd:date ;
    dct:creator "Thomas Francart" ;
  ] ;
  dcat:distribution [
    dcat:downloadURL <http://linked-statistics.github.io/xkos/xkos-best-practices-conformance-shapes.ttl> ;
    dcat:mediaType <https://www.iana.org/assignments/media-types/text/turtle> ;
  ] ;
  dcat:contactPoint <https://github.com/linked-statistics/xkos/> ;
  dct:publisher "DDi Alliance https://www.ddialliance.org/" ;  
  dcat:keyword "XKOS", "SKOS", "Statistical classifications" ;
  dct:issued "2023-01-20"^^xsd:date ;
  dct:creator "Thomas Francart" ;
  dct:language "en" ;
  dcat:landingPage <http://linked-statistics.github.io/xkos/xkos-best-practices.html#shacl-howto> ;
  # dct:isRequiredBy <https://sparnatural.eu> ;
  dct:references <http://rdf-vocabulary.ddialliance.org/xkos#>, <http://www.w3.org/2004/02/skos/core#>, <http://purl.org/dc/terms/>, <http://purl.org/dc/elements/1.1/>, <http://schema.org>, <http://data.europa.eu/eli/ontology#> ;
.

:xkosBpShapesRecommended a dcat:Dataset ;
  dct:title "XKOS best practices recommended and optional shapes" ;
  dct:description "Specifies the recommended and optional shapes defined in the <a href=\"http://linked-statistics.github.io/xkos/xkos-best-practices.html\">XKOS Best Practices guide</a>. ";
  foaf:isPrimaryTopicOf [
    dct:issued "2023-07-11"^^xsd:date ;
    dct:creator "Thomas Francart" ;
  ] ;
  dcat:distribution [
    dcat:downloadURL <http://linked-statistics.github.io/xkos/xkos-best-practices-recommended-optional-shapes.ttl> ;
    dcat:mediaType <https://www.iana.org/assignments/media-types/text/turtle> ;
  ] ;
  dcat:contactPoint <https://github.com/linked-statistics/xkos/> ;
  dct:publisher "DDi Alliance https://www.ddialliance.org/" ;  
  dcat:keyword "XKOS", "SKOS", "Statistical classifications" ;
  dct:issued "2023-01-20"^^xsd:date ;
  dct:creator "Thomas Francart" ;
  dct:language "en" ;
  dcat:landingPage <http://linked-statistics.github.io/xkos/xkos-best-practices.html#shacl-howto> ;
  # dct:isRequiredBy <https://sparnatural.eu> ;
  dct:references <http://rdf-vocabulary.ddialliance.org/xkos#>, <http://www.w3.org/2004/02/skos/core#>, <http://purl.org/dc/terms/>, <http://purl.org/dc/elements/1.1/>, <http://schema.org>, <http://data.europa.eu/eli/ontology#> ;
.
